Checkpoint

dualprocess/DualProcess.v
@@ -14,28 +14,45 @@ Definition initial := {| t := 5 ; r := 5 ; c1 := nil ; c2 := nil |}.
 
 Inductive netEvalR : netstate -> netstate -> Prop :=
 | Initial : (netEvalR initial initial)
-| Step1 : forall st,
-    st.(t) > 0 ->
-    (netEvalR st {| t := st.(t) - 1 ; r := st.(r) ;
-                    c1 := msg :: st.(c1) ; c2 := st.(c2) |})
-| Step2 : forall st,
-    st.(c2) <> nil ->
-    (netEvalR st {| t := st.(t) + 1 ; r := st.(r) ;
-                    c1 := st.(c1) ; c2 := (tl st.(c2)) |}).
-(*
-| Step3 : forall n1 n2 c1 c2,
-    c1 <> nil ->
-    (netEvalR n1 (Node (lvar n2 + 1)) (tl c1) c2)
-| Step4 : forall n1 n2 c1 c2,
-    lvar n2 > 0 ->
-    (netEvalR n1 (Node (lvar n2 - 1)) c1 (msg :: c2)).
-*)
-
-Theorem safety_holds: forall st st' : netstate,
+| Step1 : forall st st',
+    netEvalR st st' ->
+    st'.(t) > 0 ->
+    (netEvalR st' {| t := st'.(t) - 1 ; r := st'.(r) ;
+                     c1 := msg :: st'.(c1) ; c2 := st'.(c2) |})
+| Step2 : forall st st',
+    netEvalR st st' ->
+    st'.(c2) <> nil ->
+    (netEvalR st' {| t := st'.(t) + 1 ; r := st'.(r) ;
+                     c1 := st'.(c1) ; c2 := (tl st'.(c2)) |})
+| Step3 : forall st st',
+    netEvalR st st' ->
+    st'.(c1) <> nil ->
+    (netEvalR st' {| t := st'.(t) ; r := st'.(r) + 1 ;
+                    c1 := (tl st'.(c1)) ; c2 := st'.(c2) |})
+| Step4 : forall st st',
+    netEvalR st st' ->
+    st'.(r) > 0 ->
+    (netEvalR st' {| t := st'.(t) ; r := st'.(r) - 1 ;
+                    c1 := st'.(c1) ; c2 := (msg :: st'.(c2)) |}).
+      
+Lemma safety1_holds: forall st st' : netstate,
          (netEvalR st st') ->
          st'.(t) >= 0 /\ st'.(r) >= 0.
 Proof.
   intros st st' H. split.
-  - inversion H. omega. omega. omega.
-  - inversion H. omega. omega. omega.
+  - inversion H; omega. 
+  - inversion H; omega.
+Qed.
+
+Lemma safety2_holds : forall st st' : netstate,
+    (netEvalR st st') ->
+    (List.length st'.(c1) + List.length st'.(c2) + st'.(t) + st'.(r))  = 10.
+Proof.
+  intros. induction H; simpl.
+  - reflexivity.
+  - omega.
+  - admit. (* For this and next case, must use H0's assumption of nonempty list
+              to show that tail will reduce by 1, canceled out by + 1 in other term. *)
+  - admit.
+  - omega.
 Qed.
